theories/L6_PCPS/closure_conversion_util.v
@@ -22,8 +22,8 @@ Section Closure_conversion_util.
 
   Variable clo_tag : ctor_tag.
 
-  Lemma project_vars_length Scope Funs GFuns σ c genv Γ FVs S x y C Q :
-    project_vars clo_tag Scope Funs GFuns σ c genv Γ FVs S x y C Q ->
+  Lemma project_vars_length Scope Funs GFuns c genv Γ FVs S x y C Q :
+    project_vars clo_tag Scope Funs GFuns c genv Γ FVs S x y C Q ->
     @List.length var x = @List.length var y.
   Proof.
     intros Hp; induction Hp; eauto. simpl; congruence.
@@ -58,10 +58,10 @@ Section Closure_conversion_util.
         rewrite Setminus_Empty_set_neut_r in H
     end.
 
-  Lemma project_var_occurs_free_ctx_Included Scope Funs GFuns σ c genv Γ FVs S x y C Q F e:
-    project_var clo_tag Scope Funs GFuns σ c genv Γ FVs S x y C Q ->
+  Lemma project_var_occurs_free_ctx_Included Scope Funs GFuns c genv Γ FVs S x y C Q F e:
+    project_var clo_tag Scope Funs GFuns c genv Γ FVs S x y C Q ->
     (occurs_free e) \subset (F :|: [set y]) ->
-    (Scope :|: (image σ ((Funs \\ Scope) :|: GFuns) :|: image genv (Funs \\ Scope)) :|: [set Γ]) \subset F ->
+    (Scope :|: (((Funs \\ Scope) :|: GFuns) :|: image genv (Funs \\ Scope)) :|: [set Γ]) \subset F ->
     (occurs_free (C |[ e ]|)) \subset F. 
   Proof with now eauto with Ensembles_DB functions_BD. 
     intros Hproj Hinc1 Hinc2. inv Hproj.
@@ -73,12 +73,10 @@ Section Closure_conversion_util.
       rewrite occurs_free_Econstr, !FromList_cons, FromList_nil,
       Union_Empty_set_neut_r.
       eapply Union_Included.
-      + rewrite image_Union in Hinc2.
-        eapply Included_trans; [| now apply Hinc2 ].
+      + eapply Included_trans; [| now apply Hinc2 ].
         eapply Union_Included.
         eapply Included_Union_preserv_l. eapply Included_Union_preserv_r. do 2 eapply Included_Union_preserv_l.
-        eapply Singleton_Included. eapply In_image. constructor; eauto.
-
+        eapply Singleton_Included. constructor; eauto.
         eapply Included_Union_preserv_l. do 2 eapply Included_Union_preserv_r. 
         eapply Singleton_Included. eapply In_image. constructor; eauto.
       + eauto with Ensembles_DB.
@@ -88,8 +86,7 @@ Section Closure_conversion_util.
       rewrite FromList_singleton. rewrite !Setminus_Union_distr.
       rewrite Setminus_Same_set_Empty_set, Union_Empty_set_neut_r.
       eapply Union_Included.
-      + rewrite image_Union in Hinc2.
-        eapply Included_trans; [| now apply Hinc2 ].
+      + eapply Included_trans; [| now apply Hinc2 ].
         eauto 10 with Ensembles_DB functions_BD.        
       + eauto with Ensembles_DB.
     - simpl. rewrite occurs_free_Eproj.
@@ -99,11 +96,11 @@ Section Closure_conversion_util.
   Qed.
 
   
-  Lemma project_vars_occurs_free_ctx_Included Scope Funs GFuns σ c Γ genv
+  Lemma project_vars_occurs_free_ctx_Included Scope Funs GFuns c Γ genv
     FVs S xs xs' C S' F e:
-    project_vars clo_tag Scope Funs GFuns σ c genv Γ FVs S xs xs' C S' ->
+    project_vars clo_tag Scope Funs GFuns c genv Γ FVs S xs xs' C S' ->
     (occurs_free e) \subset (F :|: (FromList xs')) ->
-    (Scope :|: (image σ (Funs \\ Scope :|: GFuns) :|: image genv (Funs \\ Scope)) :|: [set  Γ]) \subset F ->
+    (Scope :|: ((Funs \\ Scope :|: GFuns) :|: image genv (Funs \\ Scope)) :|: [set  Γ]) \subset F ->
     occurs_free (C |[ e ]|) \subset F. 
   Proof. 
     intros Hproj. revert F.
@@ -115,10 +112,10 @@ Section Closure_conversion_util.
       eapply Included_trans. eassumption. now apply Included_Union_l.
   Qed.
 
-  Lemma project_var_occurs_free_ctx_alt_Included Scope Funs GFuns σ c genv Γ FVs S x y C Q F e:
-    project_var clo_tag Scope Funs GFuns σ c genv Γ FVs S x y C Q ->
+  Lemma project_var_occurs_free_ctx_alt_Included Scope Funs GFuns c genv Γ FVs S x y C Q F e:
+    project_var clo_tag Scope Funs GFuns c genv Γ FVs S x y C Q ->
     (occurs_free e) \subset (F :|: [set y]) ->
-    (Scope :|: ((image σ ([set x] :&: (Funs \\ Scope :|: GFuns)) :|: image genv (Funs \\ Scope))) :|: [set Γ]) \subset F ->
+    (Scope :|: ((([set x] :&: (Funs \\ Scope :|: GFuns)) :|: image genv (Funs \\ Scope))) :|: [set Γ]) \subset F ->
     (occurs_free (C |[ e ]|)) \subset F. 
   Proof with now eauto with Ensembles_DB functions_BD. 
     intros Hproj Hinc1 Hinc2. inv Hproj.
@@ -132,7 +129,7 @@ Section Closure_conversion_util.
       eapply Union_Included.
       + eapply Included_trans; [| now apply Hinc2 ].
         eapply Union_Included; sets. eapply Singleton_Included. left. right. left.
-        eapply In_image. constructor; eauto. left; constructor; eauto.
+        constructor; eauto. left; constructor; eauto.
         eapply Singleton_Included. left. right. right. 
         eapply In_image. constructor; eauto.        
       + eauto with Ensembles_DB.
@@ -145,7 +142,7 @@ Section Closure_conversion_util.
       + eapply Included_trans; [| now apply Hinc2 ].
         eapply Setminus_Included_Included_Union.
         eapply Singleton_Included. left. left. right. left.
-        eapply In_image. econstructor; eauto.
+        econstructor; eauto.
       + eauto with Ensembles_DB.
     - simpl. rewrite occurs_free_Eproj.
       eapply Union_Included.
@@ -154,11 +151,11 @@ Section Closure_conversion_util.
   Qed.
 
   
-  Lemma project_vars_occurs_free_ctx_alt_Included Scope Funs GFuns σ c genv Γ
+  Lemma project_vars_occurs_free_ctx_alt_Included Scope Funs GFuns c genv Γ
         FVs S xs xs' C S' F e:
-    project_vars clo_tag Scope Funs GFuns σ c genv Γ FVs S xs xs' C S' ->
+    project_vars clo_tag Scope Funs GFuns c genv Γ FVs S xs xs' C S' ->
     Included _ (occurs_free e) (Union _ F (FromList xs')) ->
-    Included _ (Scope :|: (Union _ (image σ (FromList xs :&: (Funs \\ Scope :|: GFuns)) :|: image genv (Funs \\ Scope)) (Singleton _ Γ))) F ->
+    Included _ (Scope :|: (Union _ ((FromList xs :&: (Funs \\ Scope :|: GFuns)) :|: image genv (Funs \\ Scope)) (Singleton _ Γ))) F ->
     Included _ (occurs_free (C |[ e ]|)) F. 
   Proof. 
     intros Hproj. revert F.
@@ -170,26 +167,26 @@ Section Closure_conversion_util.
       eapply Included_trans. eapply Included_trans; [| eapply Hinc2 ]; sets.
       eapply Included_Union_compat; sets.
       eapply Included_Union_compat; sets.
-      eapply Included_Union_compat; sets. eapply image_monotonic.
+      eapply Included_Union_compat; sets.
       eapply Included_Intersection_compat; sets. sets.
       eapply Included_trans; [| eassumption ].
       rewrite !Union_assoc.  eapply Included_Union_compat; sets.
       eapply Included_Union_compat; sets.
-      eapply Included_Union_compat; sets. eapply image_monotonic.
+      eapply Included_Union_compat; sets.
       eapply Included_Intersection_compat; sets.
   Qed.
 
   
-  Lemma project_var_In_Union Scope Funs GFuns σ c genv Γ FVs S x x' C S' :
-    project_var clo_tag Scope Funs GFuns σ c genv Γ FVs S x x' C S' ->
+  Lemma project_var_In_Union Scope Funs GFuns c genv Γ FVs S x x' C S' :
+    project_var clo_tag Scope Funs GFuns c genv Γ FVs S x x' C S' ->
     x \in (Scope :|: Funs :|: GFuns :|: FromList FVs).
   Proof.
     intros Hvar. inv Hvar; eauto.
     right. eapply nthN_In. eassumption.
   Qed.
 
-  Lemma project_vars_In_Union Scope Funs GFuns σ c genv Γ FVs S xs xs' C S' :
-    project_vars clo_tag Scope Funs GFuns σ c genv Γ FVs S xs xs' C S' ->
+  Lemma project_vars_In_Union Scope Funs GFuns c genv Γ FVs S xs xs' C S' :
+    project_vars clo_tag Scope Funs GFuns c genv Γ FVs S xs xs' C S' ->
     (FromList xs) \subset (Scope :|: Funs :|: GFuns :|: FromList FVs).
   Proof.
     intros Hvar. induction Hvar; eauto.
@@ -261,201 +258,6 @@ Section Closure_conversion_util.
     - eapply Included_trans. eassumption. sets.
   Qed.
 
-  (** * Lemmas about [make_closures] *)
-
-  Lemma make_closures_free_set_Included B S Γ C σ  S' :
-    make_closures clo_tag B S Γ C σ S' ->
-    S' \subset S.
-  Proof. 
-    intros Hmc. induction Hmc.
-    - now apply Included_refl.
-    - eapply Included_trans. eassumption.
-      now apply Setminus_Included.
-  Qed.
-
-  Lemma make_closures_image_Included B S Γ C σ S' :
-    make_closures clo_tag B S Γ C σ S' ->
-    Included _ (image σ (name_in_fundefs B)) (S \\ S').
-  Proof. 
-    intros Hmc. induction Hmc.
-    - rewrite image_Empty_set. apply Included_Empty_set.
-    - simpl. subst. 
-      rewrite image_Union, image_Singleton.
-      apply Union_Included. apply Singleton_Included.
-      constructor; eauto. eapply make_closures_free_set_Included in Hmc.
-      now intros Hc; eapply Hmc; eauto. 
-      eapply Included_trans. eassumption.
-      now eauto with Ensembles_DB.
-  Qed.
-
-  Lemma make_closures_image_eq B S Γ C σ S' :
-    unique_functions B ->
-    make_closures clo_tag B S Γ C σ S' ->
-    (image σ (name_in_fundefs B)) <--> (S \\ S').
-  Proof. 
-    intros Hun Hmc. induction Hmc.
-    - rewrite image_Empty_set, Setminus_Same_set_Empty_set. reflexivity.
-    - simpl. subst. 
-      rewrite image_Union, image_Singleton.
-      inv Hun. rewrite IHHmc; [| eassumption ].
-      rewrite Setminus_Union, (Union_commut [set _] S'), <- Setminus_Union. 
-      rewrite Union_Setminus_Included, Union_Same_set. reflexivity.                                                         
-      eapply Singleton_Included. constructor. eassumption.
-      eapply make_closures_free_set_Included in Hmc.
-      now intros Hc; eapply Hmc; eauto.
-      tci. reflexivity.
-  Qed.
-
-  Lemma make_closures_image_set B S Γ C σ S' P  :
-    make_closures clo_tag B S Γ C σ S' ->
-    image σ P \subset image σ (P \\ name_in_fundefs B) :|: (S \\ S').
-  Proof.
-    intros Hmc. revert P. induction Hmc; intros P.
-    - simpl. rewrite Setminus_Empty_set_neut_r, Setminus_Same_set_Empty_set, Union_Empty_set_neut_r.
-      reflexivity.
-    - simpl. subst.
-      eapply Included_trans. eapply image_monotonic.
-      eapply Included_Union_Setminus with (s2 := [set f]); tci.
-      rewrite image_Union, image_Singleton.
-      eapply Union_Included.
-      + eapply Included_trans. eapply IHHmc.
-        eapply Union_Included. 
-        eapply Included_Union_preserv_l. eapply image_monotonic.
-        now sets.
-        now sets.
-      + eapply Singleton_Included. right. constructor; eauto.
-        eapply make_closures_free_set_Included in Hmc.
-        now intros Hc; eapply Hmc; eauto.
-  Qed.
-
-  Lemma make_closures_image_Disjoint B S Γ C σ  S' :
-    make_closures clo_tag B S Γ C σ S' ->
-    Disjoint _ (image σ (name_in_fundefs B)) S'.
-  Proof.
-    intros Hc. constructor. intros x H1. inv H1.
-    eapply make_closures_image_Included in H; [| eassumption ].
-    now inv H.
-  Qed.
-
-  Lemma make_closures_injective GFuns B S Γ C σ S' :
-    Disjoint _ S (name_in_fundefs B) ->
-    Disjoint _ S (image σ GFuns) ->
-    injective_subdomain GFuns σ ->
-    make_closures clo_tag B S Γ C σ S' ->
-    injective_subdomain (name_in_fundefs B :|: GFuns) σ.
-  Proof.
-    revert GFuns S Γ C σ S'; induction B; intros GFuns S Γ C σ S' Hd Hd' Hinj Hmc.
-    - simpl. inv Hmc.
-      rewrite <- Union_assoc. eapply injective_subdomain_Union.
-      + eapply injective_subdomain_Singleton.
-      + eapply IHB; [| | | eassumption ].
-        now eapply Disjoint_Included; [| | eapply Hd ]; sets.
-        sets.
-        eassumption.
-      + rewrite image_Singleton, image_Union.
-        eapply Union_Disjoint_r.
-        eapply Disjoint_Included_r.
-        eapply make_closures_image_Included. eassumption. now sets.
-        eapply Disjoint_Included_l; [| eassumption ].
-        eapply Singleton_Included. eassumption.
-    - simpl. rewrite Union_Empty_set_neut_l. eassumption.
-  Qed.
-
-  Lemma make_closures_occurs_free_ctx_Included B S Γ C f S' F e:
-    unique_functions B ->
-    make_closures clo_tag B S Γ C f S'  ->
-    Included _ (occurs_free e) (Union _ F (name_in_fundefs B)) ->
-    (S \\ S') :|: [set Γ] \subset F ->
-    Included _ (occurs_free (C |[ e ]|)) F. 
-  Proof with now eauto with Ensembles_DB functions_BD. 
-    intros Hun Hmc. revert F.
-    induction Hmc; intros F Hinc1 Hinc2;
-    simpl in *; repeat normalize_sets; (repeat normalize_occurs_free).
-    - eassumption.
-    - repeat normalize_sets.
-      apply Union_Included. apply Union_Included.
-      eapply Included_trans; [| eassumption ].
-      eapply Singleton_Included. constructor; eauto. constructor; eauto.
-      eapply make_closures_free_set_Included in Hmc. intros Hc. eapply Hmc.
-      eassumption. now constructor.
-      now eauto with Ensembles_DB. 
-      eapply Setminus_Included_Included_Union.
-      inv Hun. eapply IHHmc.
-      eassumption. 
-      eapply Included_trans; [ eapply Hinc1 |]...
-      eapply Included_trans; [| eapply Included_Union_l ].
-      eapply Included_trans; [| eassumption ]...
-  Qed.
-
-  (** * Lemmas about [make_closure_names] *)
-
-  Lemma make_closure_names_free_set_Included B S σ  S' :
-    make_closure_names B S σ S' ->
-    S' \subset S.
-  Proof. 
-    intros Hmc. induction Hmc.
-    - now apply Included_refl.
-    - eapply Included_trans. eassumption.
-      now apply Setminus_Included.
-  Qed.
-
-
-  Lemma make_closure_names_image_eq B S σ S' :
-    unique_functions B ->
-    make_closure_names B S σ S' ->
-    (image σ (name_in_fundefs B)) <--> (S \\ S').
-  Proof. 
-    intros Hun Hmc. induction Hmc.
-    - rewrite image_Empty_set, Setminus_Same_set_Empty_set. reflexivity.
-    - simpl. subst. 
-      rewrite image_Union, image_Singleton.
-      inv Hun. rewrite IHHmc; [| eassumption ]. 
-      rewrite Setminus_Union, (Union_commut [set _] S'), <- Setminus_Union. 
-      rewrite Union_Setminus_Included, Union_Same_set. reflexivity.                                                         apply Singleton_Included. constructor. eassumption.
-      eapply make_closure_names_free_set_Included in Hmc.
-      now intros Hc; eapply Hmc; eauto.
-      tci. reflexivity.
-  Qed.
-
-  Lemma make_closure_names_image_Included B S σ S' :
-    make_closure_names B S σ S' ->
-    Included _ (image σ (name_in_fundefs B)) (S \\ S').
-  Proof. 
-    intros Hmc. induction Hmc.
-    - rewrite image_Empty_set. apply Included_Empty_set.
-    - simpl. subst. 
-      rewrite image_Union, image_Singleton.
-      apply Union_Included. apply Singleton_Included.
-      constructor; eauto. eapply make_closure_names_free_set_Included in Hmc.
-      now intros Hc; eapply Hmc; eauto. 
-      eapply Included_trans. eassumption.
-      now eauto with Ensembles_DB.
-  Qed.
-
-  Lemma make_closure_names_injective GFuns B S σ S' :
-    Disjoint _ S (name_in_fundefs B) ->
-    Disjoint _ S (image σ GFuns) ->
-    injective_subdomain GFuns σ ->
-    make_closure_names B S σ S' ->
-    injective_subdomain (name_in_fundefs B :|: GFuns) σ.
-  Proof.
-    revert GFuns S σ S'; induction B; intros GFuns S σ S' Hd Hd' Hinj Hmc.
-    - simpl. inv Hmc.
-      rewrite <- Union_assoc. eapply injective_subdomain_Union.
-      + eapply injective_subdomain_Singleton.
-      + eapply IHB; [| | | eassumption ].
-        now eapply Disjoint_Included; [| | eapply Hd ]; sets.
-        sets.
-        eassumption.
-      + rewrite image_Singleton, image_Union.
-        eapply Union_Disjoint_r. eapply Disjoint_Included_r.
-        eapply make_closure_names_image_Included. eassumption. now sets.
-        eapply Disjoint_Included_l; [| eassumption ].
-        eapply Singleton_Included. eassumption.
-    - simpl. rewrite Union_Empty_set_neut_l. eassumption.
-  Qed.
-
-
   (** * Lemmas about [extend_fundefs'] *)
   
   Lemma extend_fundefs'_get_s f B x z :
@@ -517,8 +319,8 @@ Section Closure_conversion_util.
   Qed.
 
   
-  Lemma project_var_free_funs_in_exp Scope Funs GFuns σ c genv Γ FVs S x x' C S' B e:
-    project_var clo_tag Scope Funs GFuns σ c genv Γ FVs S x x' C S' ->
+  Lemma project_var_free_funs_in_exp Scope Funs GFuns c genv Γ FVs S x x' C S' B e:
+    project_var clo_tag Scope Funs GFuns c genv Γ FVs S x x' C S' ->
     (funs_in_exp B (C |[ e ]|) <-> funs_in_exp B e).
   Proof. 
     intros Hvar; inv Hvar; [ split; now eauto | |  |];
@@ -528,31 +330,22 @@ Section Closure_conversion_util.
       constructor. now constructor. 
   Qed.
 
-  Lemma project_vars_free_funs_in_exp Scope Funs GFuns σ c genv Γ FVs S xs xs' C S' B e:
-    project_vars clo_tag Scope Funs GFuns σ c genv Γ FVs S xs xs' C S' ->
+  Lemma project_vars_free_funs_in_exp Scope Funs GFuns c genv Γ FVs S xs xs' C S' B e:
+    project_vars clo_tag Scope Funs GFuns c genv Γ FVs S xs xs' C S' ->
     (funs_in_exp B (C |[ e ]|) <-> funs_in_exp B e).
   Proof. 
     intros Hvar; induction Hvar; [ now eauto |].
     rewrite <- app_ctx_f_fuse, project_var_free_funs_in_exp; eassumption.
   Qed.
 
-  Lemma make_closures_funs_in_exp B S Γ C σ S' B' e:
-    make_closures clo_tag B S Γ C σ S'  ->
-    (funs_in_exp B' (C |[ e ]|) <-> funs_in_exp B' e).
-  Proof.
-    intros Hmc; induction Hmc;
-    [ split; now eauto | ].
-    rewrite <- IHHmc. split; eauto; intros Hf; [ now inv Hf | now constructor ].
-  Qed.
-
-  Lemma closure_conversion_fundefs_Same_set_image σ c Funs GFuns FVs B1 B2  :
-    Closure_conversion_fundefs clo_tag Funs GFuns σ c FVs B1 B2 ->
-    Same_set _ (image σ (name_in_fundefs B1)) (name_in_fundefs B2).
+  Lemma closure_conversion_fundefs_Same_set_image c Funs GFuns FVs B1 B2  :
+    Closure_conversion_fundefs clo_tag Funs GFuns c FVs B1 B2 ->
+    Same_set _ ((name_in_fundefs B1)) (name_in_fundefs B2).
   Proof. 
     intros Hcc. induction Hcc.  
-    - simpl. rewrite image_Union, image_Singleton, IHHcc.
+    - simpl. rewrite  IHHcc.
       apply Same_set_refl.
-    - simpl. rewrite image_Empty_set. apply Same_set_refl.
+    - simpl. apply Same_set_refl.
   Qed.
 
 
@@ -575,33 +368,33 @@ Section Closure_conversion_util.
   Qed. 
     
   Lemma Closure_conversion_occurs_free_pre_Included :
-    (forall e Scope Funs GFuns {_ : Decidable GFuns} σ c genv Γ FVs e' C 
-       (Hcc : Closure_conversion clo_tag Scope Funs GFuns σ c genv Γ FVs e e' C),
+    (forall e Scope Funs GFuns {_ : Decidable GFuns} c genv Γ FVs e' C 
+       (Hcc : Closure_conversion clo_tag Scope Funs GFuns c genv Γ FVs e e' C),
         (occurs_free e) \subset (Scope :|: Funs :|: GFuns :|: FromList FVs)).
   Proof with now eauto with Ensembles_DB functions_BD.
     induction e using exp_ind'; intros; inv Hcc; normalize_occurs_free.
     - eapply Union_Included. eapply project_vars_In_Union. eassumption.
-      eapply IHe in H16. eapply Setminus_Included_Included_Union.
+      eapply IHe in H15. eapply Setminus_Included_Included_Union.
       eapply Included_trans. eassumption. repeat (eapply Union_Included; sets).
       tci. 
     - eapply Singleton_Included. eapply project_var_In_Union. eassumption.
     - eapply Union_Included. 
       eapply Singleton_Included. eapply project_var_In_Union. eassumption.
-      inv H14. destruct H3 as [Hfeq [C1 [e1 [Hceq Hcc]]]].
+      inv H13. destruct H3 as [Hfeq [C1 [e1 [Hceq Hcc]]]].
       eapply Union_Included.
       eapply IHe; eassumption.
       eapply IHe0; eauto. econstructor; eauto.
     - eapply Union_Included. eapply Singleton_Included. eapply project_var_In_Union. eassumption.
-      eapply IHe in H17. eapply Setminus_Included_Included_Union.
+      eapply IHe in H16. eapply Setminus_Included_Included_Union.
       eapply Included_trans. eassumption. repeat (eapply Union_Included; sets). tci.
     - eapply Union_Included. rewrite <- FromList_cons. eapply project_vars_In_Union. eassumption.
-      eapply IHe in H20. eapply Setminus_Included_Included_Union.
+      eapply IHe in H19. eapply Setminus_Included_Included_Union.
       eapply Included_trans. eassumption. repeat (eapply Union_Included; sets). tci.
     - eapply Union_Included.
       eapply Included_trans. eapply Setminus_eq_Included; [| eassumption ]. tci.
       eapply Union_Included. sets.
       eapply project_vars_In_Union. eassumption.
-      eapply IHe in H21; tci. eapply Setminus_Included_Included_Union.
+      eapply IHe in H19; tci. eapply Setminus_Included_Included_Union.
       eapply Included_trans. eassumption.
       eapply Union_Included; sets.
       eapply Union_Included; sets.
@@ -611,21 +404,21 @@ Section Closure_conversion_util.
     - eapply Included_trans; [| eapply project_vars_In_Union; eauto ].
       normalize_sets...
     - eapply Union_Included. eapply project_vars_In_Union. eassumption.
-      eapply IHe in H16. eapply Setminus_Included_Included_Union.
+      eapply IHe in H15. eapply Setminus_Included_Included_Union.
       eapply Included_trans. eassumption. repeat (eapply Union_Included; sets).
       tci.
     - eapply Singleton_Included. eapply project_var_In_Union. eassumption.
   Qed.  
   
   Lemma Closure_conversion_occurs_free_Included_mut :
-    (forall e Scope Funs GFuns σ c genv Γ FVs e' C 
-       (Hcc : Closure_conversion clo_tag Scope Funs GFuns σ c genv Γ FVs e e' C)
+    (forall e Scope Funs GFuns c genv Γ FVs e' C 
+       (Hcc : Closure_conversion clo_tag Scope Funs GFuns c genv Γ FVs e e' C)
        (Hun: fundefs_names_unique e),
-        occurs_free (C |[ e' ]|) \subset (Scope :|: (image σ (Funs \\ Scope :|: GFuns) :|: image genv (Funs \\ Scope)) :|: [set Γ])) /\
-    (forall B Bg GFuns σ c FVs B'
-       (Hcc: Closure_conversion_fundefs clo_tag Bg GFuns σ c FVs B B')
+        occurs_free (C |[ e' ]|) \subset (Scope :|: ((Funs \\ Scope :|: GFuns) :|: image genv (Funs \\ Scope)) :|: [set Γ])) /\
+    (forall B Bg GFuns c FVs B'
+       (Hcc: Closure_conversion_fundefs clo_tag Bg GFuns c FVs B B')
        (Hun: fundefs_names_unique_fundefs B),
-       occurs_free_fundefs B' \subset (image σ (name_in_fundefs Bg :|: GFuns) \\ (name_in_fundefs B'))).
+       occurs_free_fundefs B' \subset ((name_in_fundefs Bg :|: GFuns) \\ (name_in_fundefs B'))).
   Proof with now eauto with Ensembles_DB functions_BD.
     exp_defs_induction IHe IHl IHB; intros; inv Hcc.
     - eapply project_vars_occurs_free_ctx_Included;
@@ -639,9 +432,9 @@ Section Closure_conversion_util.
       eapply Union_Included; sets.
       eapply Union_Included; eauto 10 with Ensembles_DB functions_BD.      
     - eapply project_var_occurs_free_ctx_Included;
-        [ eassumption | | now apply Included_refl ]. inv H13.
+        [ eassumption | | now apply Included_refl ]. inv H12.
       rewrite occurs_free_Ecase_nil. now apply Included_Union_r.
-    - inv H13. destruct y as [c' e'].
+    - inv H12. destruct y as [c' e'].
       inv H2. simpl in H; subst. destruct H0 as [C' [e'' [Heq Hcce]]]. simpl in Heq; subst. 
       eapply Included_trans. now eapply occurs_free_Ecase_ctx_app.
       apply Union_Included. 
@@ -693,10 +486,10 @@ Section Closure_conversion_util.
       + eapply Included_trans. eapply IHB. eassumption.
         intros f Hunf. eapply Hun. now inv Hunf; eauto.
         eapply Setminus_Included_Included_Union.
-        rewrite image_Union. rewrite closure_conversion_fundefs_Same_set_image; [| eassumption ].
+        rewrite closure_conversion_fundefs_Same_set_image; [| eassumption ].
         eapply Union_Included; sets.
-        eapply Included_trans. eapply image_monotonic. eapply add_global_funs_included_r; eauto.
-        rewrite !image_Union. rewrite closure_conversion_fundefs_Same_set_image; [| eassumption ].
+        eapply Included_trans. eapply add_global_funs_included_r; eauto.
+        rewrite closure_conversion_fundefs_Same_set_image; [| eassumption ].
         eauto 20 with Ensembles_DB. 
       + eapply Setminus_Included_Included_Union.
         eapply Included_trans. eapply IHe. eassumption.
@@ -704,17 +497,16 @@ Section Closure_conversion_util.
         eapply Union_Included; sets.
         eapply Union_Included. xsets.
         eapply Union_Included; sets.
-        * eapply Included_trans. eapply image_monotonic. eapply Included_Union_compat; [| reflexivity ].
+        * eapply Included_trans. eapply Included_Union_compat; [| reflexivity ].
           eapply Setminus_Setminus_Included. tci.
           rewrite Setminus_Union_distr.
           rewrite <- !Union_assoc.
           rewrite (Union_Same_set (name_in_fundefs _ \\ Scope)); sets.
-          rewrite !image_Union.
           eapply Union_Included; eauto 10 with Ensembles_DB.
           eapply Union_Included; eauto 10 with Ensembles_DB.
           rewrite closure_conversion_fundefs_Same_set_image; [| eassumption ]. xsets.
-          eapply Included_trans. eapply image_monotonic. eapply add_global_funs_included_r; eauto.
-          rewrite !image_Union. rewrite closure_conversion_fundefs_Same_set_image; [| eassumption ].
+          eapply Included_trans. eapply add_global_funs_included_r; eauto.
+          rewrite closure_conversion_fundefs_Same_set_image; [| eassumption ].
           eauto 20 with Ensembles_DB.
         * eapply Included_trans. eapply extend_fundefs'_image_Included'.
           eapply Union_Included; sets.
@@ -781,15 +573,15 @@ Section Closure_conversion_util.
 
   
   Lemma Closure_conversion_occurs_free_Included_alt_mut :
-    (forall e Scope Funs GFuns σ c genv Γ FVs e' C 
-       (Hcc : Closure_conversion clo_tag Scope Funs GFuns σ c genv Γ FVs e e' C)
+    (forall e Scope Funs GFuns c genv Γ FVs e' C 
+       (Hcc : Closure_conversion clo_tag Scope Funs GFuns c genv Γ FVs e e' C)
        (Hun: fundefs_names_unique e),
         occurs_free (C |[ e' ]|) \subset
-        Scope :|: (image σ (occurs_free e :&: (Funs \\ Scope :|: GFuns)) :|: image genv (Funs \\ Scope)) :|: [set Γ]) /\
-    (forall B Bg GFuns σ c FVs B'
-       (Hcc: Closure_conversion_fundefs clo_tag Bg GFuns σ c FVs B B')
+        Scope :|: ((occurs_free e :&: (Funs \\ Scope :|: GFuns)) :|: image genv (Funs \\ Scope)) :|: [set Γ]) /\
+    (forall B Bg GFuns c FVs B'
+       (Hcc: Closure_conversion_fundefs clo_tag Bg GFuns c FVs B B')
        (Hun: fundefs_names_unique_fundefs B),
-        occurs_free_fundefs B' \subset image σ (occurs_free_fundefs B :&: (name_in_fundefs Bg :|: GFuns))).
+        occurs_free_fundefs B' \subset (occurs_free_fundefs B :&: (name_in_fundefs Bg :|: GFuns))).
   Proof with now eauto with Ensembles_DB functions_BD.
     exp_defs_induction IHe IHl IHB; intros; inv Hcc.
     - eapply project_vars_occurs_free_ctx_alt_Included; [ eassumption | | sets ].
@@ -802,7 +594,6 @@ Section Closure_conversion_util.
       eapply Union_Included; xsets.
       
       do 3 eapply Included_Union_preserv_l. eapply Included_Union_preserv_r. eapply Included_Union_preserv_l.
-      eapply image_monotonic.
       rewrite <- Intersection_Setmius_Disjoint with (S2 := [set v]). eapply Included_Intersection_compat; sets.
       sets.
 
@@ -810,11 +601,11 @@ Section Closure_conversion_util.
       eapply Union_Included; sets.
       normalize_occurs_free.  eapply Union_Included; sets. 
       eapply Included_Union_preserv_l. eapply Included_Union_preserv_r. eapply Included_Union_preserv_l.
-      eapply image_monotonic. eapply Included_Intersection_compat; sets.
-    - eapply project_var_occurs_free_ctx_alt_Included; [ eassumption | | sets ]. inv H13.
+      eapply Included_Intersection_compat; sets.
+    - eapply project_var_occurs_free_ctx_alt_Included; [ eassumption | | sets ]. inv H12.
       repeat normalize_occurs_free. sets.
       normalize_occurs_free... 
-    - inv H13. destruct y as [c' e'].
+    - inv H12. destruct y as [c' e'].
       inv H2. simpl in H; subst. destruct H0 as [C' [e'' [Heq Hcce]]]. simpl in Heq; subst. 
       eapply Included_trans. now eapply occurs_free_Ecase_ctx_app.
       apply Union_Included. 
@@ -825,13 +616,13 @@ Section Closure_conversion_util.
         eapply Union_Included; sets.
         eapply Union_Included; sets.        
         do 2 eapply Included_Union_preserv_l. eapply Included_Union_preserv_r. eapply Included_Union_preserv_l.
-        eapply image_monotonic. eapply Included_Intersection_compat; sets.
+        eapply Included_Intersection_compat; sets.
 
         eapply Union_Included; sets.
         eapply Union_Included; sets.
         eapply Union_Included; sets.
         eapply Included_Union_preserv_l. eapply Included_Union_preserv_r. eapply Included_Union_preserv_l.
-        eapply image_monotonic. eapply Included_Intersection_compat; sets.
+        eapply Included_Intersection_compat; sets.
       + eapply Included_trans. eapply IHl. econstructor; eauto.
         intros f Hfin. eapply Hun. inv Hfin. econstructor. eassumption. right. eassumption.
         normalize_occurs_free.
@@ -839,7 +630,7 @@ Section Closure_conversion_util.
         eapply Union_Included; sets.
         eapply Union_Included; sets.
         eapply Included_Union_preserv_l. eapply Included_Union_preserv_r. eapply Included_Union_preserv_l.
-        eapply image_monotonic. eapply Included_Intersection_compat; sets.
+        eapply Included_Intersection_compat; sets.
     - eapply project_var_occurs_free_ctx_alt_Included; [ eassumption | | sets ].
       repeat normalize_occurs_free.
       apply Union_Included. now eauto with Ensembles_DB. eapply Setminus_Included_Included_Union.
@@ -849,7 +640,6 @@ Section Closure_conversion_util.
       eapply Union_Included; [| sets ]. now sets. 
       eapply Union_Included; sets.
       do 3 eapply Included_Union_preserv_l. eapply Included_Union_preserv_r. eapply Included_Union_preserv_l.
-      eapply image_monotonic.
       rewrite <- Intersection_Setmius_Disjoint with (S2 := [set v]). eapply Included_Intersection_compat; sets.
       now sets. now xsets. 
       eapply Union_Included; sets.
@@ -857,7 +647,7 @@ Section Closure_conversion_util.
       normalize_occurs_free.
       eapply Union_Included; sets.      
       eapply Included_Union_preserv_l. eapply Included_Union_preserv_r. eapply Included_Union_preserv_l.
-      eapply image_monotonic. eapply Included_Intersection_compat; sets.
+      eapply Included_Intersection_compat; sets.
     - eapply project_vars_occurs_free_ctx_alt_Included; [ eassumption | | normalize_sets; normalize_occurs_free; sets ].
       repeat normalize_occurs_free. repeat normalize_sets. 
       eapply Union_Included; sets.
@@ -872,14 +662,13 @@ Section Closure_conversion_util.
       eapply Union_Included; sets.
       eapply Union_Included; sets. now xsets. eapply Union_Included; sets.
       do 5 eapply Included_Union_preserv_l. eapply Included_Union_preserv_r. eapply Included_Union_preserv_l.
-      eapply image_monotonic.
       rewrite <- Intersection_Setmius_Disjoint with (S2 := [set x]). eapply Included_Intersection_compat; sets.
       now sets. now xsets. 
       eapply Union_Included; sets.
       eapply Union_Included; sets.
       eapply Union_Included; sets.
       eapply Included_Union_preserv_l. eapply Included_Union_preserv_r. eapply Included_Union_preserv_l.
-      eapply image_monotonic. eapply Included_Intersection_compat; sets.
+      eapply Included_Intersection_compat; sets.
     - simpl. rewrite <- app_ctx_f_fuse. 
       eapply project_vars_occurs_free_ctx_alt_Included; [ eassumption | | ].  
       + simpl. repeat normalize_occurs_free.
@@ -888,11 +677,11 @@ Section Closure_conversion_util.
         * eapply Setminus_Included_Included_Union. eapply Included_trans.
           eapply IHB. eassumption.  intros f Hfin. inv Hfin; subst; now eauto.
           eapply Included_trans. 
-          eapply image_monotonic. eapply Included_Intersection_compat. reflexivity.
+          eapply Included_Intersection_compat. reflexivity.
           eapply Union_Included; [| eapply add_global_funs_included_r; eassumption]. sets.
           do 3 eapply Included_Union_preserv_l. eapply Included_Union_preserv_r. eapply Included_Union_preserv_l. 
           rewrite Intersection_commut. rewrite Intersection_Union_Disjoint. 
-          rewrite Intersection_commut. eapply image_monotonic.
+          rewrite Intersection_commut. 
           eapply Included_Intersection_compat; sets. eapply occurs_free_fundefs_name_in_fundefs_Disjoint; eauto.
         * { do 2 eapply Setminus_Included_Included_Union. eapply Included_trans. eapply IHe. eassumption.
             intros f Hfin. eapply Hun. now constructor.
@@ -907,13 +696,12 @@ Section Closure_conversion_util.
                 eapply Setminus_Setminus_Included. tci. eapply Union_Included; sets. }
               
               eapply Union_Included; [| eapply Union_Included ]; sets.
-              + eapply Included_trans. eapply image_monotonic.
+              + eapply Included_trans.
                 eapply Included_Intersection_compat. reflexivity. eapply Included_Union_compat.
                 eassumption. reflexivity.
                 eapply Included_trans
-                  with (s2 :=  image σ ((occurs_free_fundefs f2 :|: (occurs_free e \\ name_in_fundefs f2)) :&: (Funs \\ Scope :|: GFuns)) :|: name_in_fundefs B'); [| xsets ].
+                  with (s2 :=  ((occurs_free_fundefs f2 :|: (occurs_free e \\ name_in_fundefs f2)) :&: (Funs \\ Scope :|: GFuns)) :|: name_in_fundefs B'); [| xsets ].
                 rewrite <- (closure_conversion_fundefs_Same_set_image) with (B2 := B'); [| eassumption ].
-                rewrite <- image_Union. eapply image_monotonic.
                 rewrite Union_Intersection_distr. eapply Included_Intersection_compat.
                 rewrite <- !Union_assoc. eapply Included_Union_preserv_r. sets.
                 rewrite <- Union_Setminus; tci; sets. 
@@ -926,7 +714,7 @@ Section Closure_conversion_util.
       + rewrite <- H1, !Union_assoc.
         normalize_occurs_free. eapply Included_Union_compat; sets.
         eapply Included_Union_compat; sets.
-        eapply Included_Union_compat; sets. eapply image_monotonic.
+        eapply Included_Union_compat; sets. 
         eapply Included_Intersection_compat; sets. 
     - eapply project_vars_occurs_free_ctx_alt_Included; [ eassumption | | normalize_sets; normalize_occurs_free; sets ].
       repeat normalize_occurs_free. repeat normalize_sets. 
@@ -939,7 +727,7 @@ Section Closure_conversion_util.
       eapply Union_Included; sets.
       eapply Union_Included; sets.
       do 1 eapply Included_Union_preserv_l. eapply Included_Union_preserv_r. eapply Included_Union_preserv_l.
-      eapply image_monotonic. eapply Included_Intersection_compat; sets.
+      eapply Included_Intersection_compat; sets.
     - eapply project_vars_occurs_free_ctx_alt_Included; [ eassumption | | sets ].
       repeat normalize_occurs_free.
       apply Union_Included. now eauto with Ensembles_DB. eapply Setminus_Included_Included_Union.
@@ -950,7 +738,6 @@ Section Closure_conversion_util.
       now sets.
       eapply Union_Included; [| now xsets ].
       do 3 eapply Included_Union_preserv_l. eapply Included_Union_preserv_r. eapply Included_Union_preserv_l.
-      eapply image_monotonic.
       rewrite <- Intersection_Setmius_Disjoint with (S2 := [set v]). eapply Included_Intersection_compat; sets.
       sets.
 
@@ -958,7 +745,7 @@ Section Closure_conversion_util.
       eapply Union_Included; sets. eapply Union_Included; sets.
       normalize_occurs_free. 
       eapply Included_Union_preserv_l. eapply Included_Union_preserv_r. eapply Included_Union_preserv_l.
-      eapply image_monotonic. eapply Included_Intersection_compat; sets.
+      eapply Included_Intersection_compat; sets.
     - eapply project_var_occurs_free_ctx_alt_Included; [ eassumption | | ].
       repeat normalize_occurs_free. sets.
       repeat normalize_occurs_free. sets.
@@ -971,22 +758,20 @@ Section Closure_conversion_util.
         eapply Union_Included; sets.
         eapply Union_Included; sets.  
 
-        eapply Included_trans with (s2 := image σ ((occurs_free e \\ (v |: (FromList l :|: name_in_fundefs f5))
-                                                                :|: (occurs_free_fundefs f5 \\ [set v])) :&: (name_in_fundefs Bg :|: GFuns)) :|: [set (σ v)]
+        eapply Included_trans with (s2 := ((occurs_free e \\ (v |: (FromList l :|: name_in_fundefs f5))
+                                                                :|: (occurs_free_fundefs f5 \\ [set v])) :&: (name_in_fundefs Bg :|: GFuns)) :|: [set (v)]
                                                 :|: name_in_fundefs defs'); [| sets ].
         rewrite <- (closure_conversion_fundefs_Same_set_image) with (B2 := defs'); [| eassumption ].
-        rewrite <- image_Singleton, <- !image_Union.
-        rewrite !Union_Intersection_distr. eapply image_monotonic.
+        rewrite !Union_Intersection_distr. 
         rewrite <- Intersection_Setmius_Disjoint with (S2 := FromList l); sets.
         eapply Included_Intersection_compat; sets. eapply Setminus_Included_Included_Union.
         rewrite <- !Union_assoc. rewrite <- Union_Included_Union_Setminus. sets. tci. sets. sets.
 
         eapply Included_trans. eapply image_monotonic. eapply Setminus_Included.
         eapply Included_trans. eapply extend_fundefs'_image. sets.
-      + eapply IHB in H12. eapply Setminus_Included_Included_Union. eapply Included_trans. eassumption.
+      + eapply IHB in H11. eapply Setminus_Included_Included_Union. eapply Included_trans. eassumption.
         normalize_occurs_free. 
-        rewrite <- image_Singleton, <- image_Union.
-        rewrite Union_Intersection_distr. eapply image_monotonic. eapply Included_Intersection_compat; sets.
+        rewrite Union_Intersection_distr. eapply Included_Intersection_compat; sets.
         rewrite <- !Union_assoc.
         rewrite <- Union_Setminus; tci; sets.
         intros x Hfun. inv Hfun; eauto.
@@ -996,10 +781,10 @@ Section Closure_conversion_util.
   Qed.
 
   Lemma Closure_conversion_occurs_free_fundefs_cor :
-    (forall B GFuns {Hd : Decidable GFuns} σ c FVs B'
-       (Hcc: Closure_conversion_fundefs clo_tag B GFuns σ c FVs B B')
+    (forall B GFuns {Hd : Decidable GFuns} c FVs B'
+       (Hcc: Closure_conversion_fundefs clo_tag B GFuns c FVs B B')
        (Hun: fundefs_names_unique_fundefs B),
-        occurs_free_fundefs B' \subset image σ (occurs_free_fundefs B :&: GFuns)).
+        occurs_free_fundefs B' \subset (occurs_free_fundefs B :&: GFuns)).
   Proof.
     intros. eapply Closure_conversion_occurs_free_Included_alt_mut in Hcc; eauto. 
     eapply Included_trans. eassumption.
@@ -1094,45 +879,39 @@ Section Closure_conversion_util.
 
   (** * Lemmas about [Closure_conversion_fundefs] *)
   
-  Lemma closure_conversion_fundefs_find_def σ c Bg GFuns FVs B1 B2 f t1 xs e1 :
-    injective_subdomain (name_in_fundefs B1) σ ->
-    Closure_conversion_fundefs clo_tag Bg GFuns σ c FVs B1 B2 ->
+  Lemma closure_conversion_fundefs_find_def c Bg GFuns FVs B1 B2 f t1 xs e1 :
+    Closure_conversion_fundefs clo_tag Bg GFuns c FVs B1 B2 ->
     find_def f B1 = Some (t1, xs, e1) ->
     exists Γ' C e2,
-      ~ In var (Union var (image σ (name_in_fundefs Bg :|: GFuns)) (Union _ (FromList xs) (bound_var e1))) Γ' /\
-      find_def (σ f) B2 = Some (t1, Γ' :: xs, (C |[ e2 ]|)) /\
-      Closure_conversion clo_tag (FromList xs) (name_in_fundefs Bg) (GFuns \\ (FromList xs)) σ c
+      ~ In var (Union var ((name_in_fundefs Bg :|: GFuns)) (Union _ (FromList xs) (bound_var e1))) Γ' /\
+      find_def (f) B2 = Some (t1, Γ' :: xs, (C |[ e2 ]|)) /\
+      Closure_conversion clo_tag (FromList xs) (name_in_fundefs Bg) (GFuns \\ (FromList xs)) c
                          (extend_fundefs' id Bg Γ')  Γ' FVs e1 e2 C.
   Proof.
-    intros Hinj Hcc Hdef. induction Hcc.
+    intros Hcc Hdef. induction Hcc.
     - simpl in Hdef. destruct (M.elt_eq f f0) eqn:Heq; subst.
       + inv Hdef. repeat eexists; eauto. 
         simpl. 
         intros Hc. eapply H. now eauto.
         simpl. rewrite peq_true. reflexivity.
       + edestruct IHHcc as [Γ'' [C' [e2 [Hnin [Hfind Hcc']]]]]; eauto.
-        eapply injective_subdomain_antimon. eassumption.
-        now apply Included_Union_r.
         repeat eexists; eauto. simpl. rewrite peq_false. eassumption.
-        intros Hc. eapply n. eapply Hinj; eauto.
-        right. eapply fun_in_fundefs_name_in_fundefs.
-        eapply find_def_correct. now eauto.
-        left; eauto.
+        intros Hc. now eapply n. 
     - inv Hdef.
   Qed.
 
 
   (** * Lemmas about [project_var] and [project_vars] *)
 
-  Lemma project_var_free_set_Included Scope Funs GFuns σ c genv Γ FVs x x' C S S' :
-    project_var clo_tag Scope GFuns Funs σ c genv Γ FVs S x x' C S' ->
+  Lemma project_var_free_set_Included Scope Funs GFuns c genv Γ FVs x x' C S S' :
+    project_var clo_tag Scope GFuns Funs c genv Γ FVs S x x' C S' ->
     Included _ S' S.
   Proof with now eauto with Ensembles_DB.
     intros Hproj. inv Hproj...
   Qed.
 
-  Lemma project_vars_free_set_Included Scope Funs GFuns σ c genv Γ FVs xs xs' C S S' :
-    project_vars clo_tag Scope Funs GFuns σ c genv Γ FVs S xs xs' C S' ->
+  Lemma project_vars_free_set_Included Scope Funs GFuns c genv Γ FVs xs xs' C S S' :
+    project_vars clo_tag Scope Funs GFuns c genv Γ FVs S xs xs' C S' ->
     Included _ S' S.
   Proof.
     intros Hproj. induction Hproj.
@@ -1141,9 +920,9 @@ Section Closure_conversion_util.
       eapply project_var_free_set_Included. eassumption. 
   Qed.
 
-  Lemma project_var_not_In_free_set Scope Funs GFuns σ c genv Γ FVs x x' C S S'  :
-    project_var clo_tag Scope Funs GFuns σ c genv Γ FVs S x x' C S' ->
-    Disjoint _ S (Scope :|: (image σ ((Funs \\ Scope) :|: GFuns) :|:
+  Lemma project_var_not_In_free_set Scope Funs GFuns c genv Γ FVs x x' C S S'  :
+    project_var clo_tag Scope Funs GFuns c genv Γ FVs S x x' C S' ->
+    Disjoint _ S (Scope :|: (((Funs \\ Scope) :|: GFuns) :|:
                                    ((FromList FVs) :|: ([set Γ])))) ->
     ~ In _ S' x'.
   Proof.
@@ -1154,9 +933,9 @@ Section Closure_conversion_util.
     - inv Hc; eauto.
   Qed.
 
-  Lemma project_vars_not_In_free_set Scope Funs GFuns σ c genv Γ FVs xs xs' C S S'  :
-    project_vars clo_tag Scope Funs GFuns σ c genv Γ FVs S xs xs' C S' ->
-    Disjoint _ S (Scope :|: (image σ ((Funs \\ Scope) :|: GFuns) :|:
+  Lemma project_vars_not_In_free_set Scope Funs GFuns c genv Γ FVs xs xs' C S S'  :
+    project_vars clo_tag Scope Funs GFuns c genv Γ FVs S xs xs' C S' ->
+    Disjoint _ S (Scope :|: (((Funs \\ Scope) :|: GFuns) :|:
                                    ((FromList FVs) :|: ([set Γ]))))  ->
     Disjoint _ S' (FromList xs').
   Proof.
@@ -1175,8 +954,8 @@ Section Closure_conversion_util.
         eassumption.
   Qed.
 
-  Lemma project_var_get Scope Funs GFuns σ c genv Γ FVs S1 x x' C1 S2 rho1 rho2 y:
-    project_var clo_tag Scope Funs GFuns σ c genv Γ FVs S1 x x' C1 S2 ->
+  Lemma project_var_get Scope Funs GFuns c genv Γ FVs S1 x x' C1 S2 rho1 rho2 y:
+    project_var clo_tag Scope Funs GFuns c genv Γ FVs S1 x x' C1 S2 ->
     ctx_to_rho C1 rho1 rho2 ->
     ~ In _ S1 y ->
     M.get y rho1 = M.get y rho2. 
@@ -1199,8 +978,8 @@ Section Closure_conversion_util.
       now rewrite M.gso.
   Qed.
 
-  Lemma project_vars_get Scope Funs GFuns σ c genv Γ FVs S1 xs xs' C1 S2 rho1 rho2 y:
-    project_vars clo_tag Scope Funs GFuns σ c genv Γ FVs S1 xs xs' C1 S2 ->
+  Lemma project_vars_get Scope Funs GFuns c genv Γ FVs S1 xs xs' C1 S2 rho1 rho2 y:
+    project_vars clo_tag Scope Funs GFuns c genv Γ FVs S1 xs xs' C1 S2 ->
     ctx_to_rho C1 rho1 rho2 ->
     ~ In _ S1 y ->
     M.get y rho1 = M.get y rho2. 
@@ -1218,8 +997,8 @@ Section Closure_conversion_util.
       eapply project_var_free_set_Included; eassumption.
   Qed.
 
-  Lemma project_var_get_list Scope Funs GFuns σ c genv Γ FVs S1 x x' C1 S2 rho1 rho2 ys :
-    project_var clo_tag Scope Funs GFuns σ c genv Γ FVs S1 x x' C1 S2 ->
+  Lemma project_var_get_list Scope Funs GFuns c genv Γ FVs S1 x x' C1 S2 rho1 rho2 ys :
+    project_var clo_tag Scope Funs GFuns c genv Γ FVs S1 x x' C1 S2 ->
     ctx_to_rho C1 rho1 rho2 ->
     Disjoint _ S1 (FromList ys) ->
     get_list ys rho1 = get_list ys rho2. 
@@ -1234,8 +1013,8 @@ Section Closure_conversion_util.
       intros Hc. eapply Hnin. eauto.
   Qed.
 
-  Lemma project_vars_get_list Scope Funs GFuns σ c genv Γ FVs S1 xs xs' C1 S2 rho1 rho2 ys :
-    project_vars clo_tag Scope Funs GFuns σ c genv Γ FVs S1 xs xs' C1 S2 ->
+  Lemma project_vars_get_list Scope Funs GFuns c genv Γ FVs S1 xs xs' C1 S2 rho1 rho2 ys :
+    project_vars clo_tag Scope Funs GFuns c genv Γ FVs S1 xs xs' C1 S2 ->
     ctx_to_rho C1 rho1 rho2 ->
     Disjoint _ S1 (FromList ys) ->
     get_list ys rho1 = get_list ys rho2. 
@@ -1250,23 +1029,23 @@ Section Closure_conversion_util.
       intros Hc. eapply Hnin. eauto.
   Qed.        
 
-  Lemma project_var_not_In Scope Funs GFuns σ c genv Γ FVs S x x' C S' :
+  Lemma project_var_not_In Scope Funs GFuns c genv Γ FVs S x x' C S' :
     Disjoint _ S (Union var Scope
                         (Union var (Funs :|: GFuns)
                                (Union var (FromList FVs) (Singleton var Γ)))) ->
     
-    project_var clo_tag Scope Funs GFuns σ c genv Γ FVs S x x' C S' ->
+    project_var clo_tag Scope Funs GFuns c genv Γ FVs S x x' C S' ->
     ~ In _ S x.
   Proof.
     intros Hd  Hproj. inv Hproj; intros Hin; try now eapply Hd; eauto.
     eapply nthN_In in H2. eapply Hd. eauto.
   Qed.
 
-  Lemma project_vars_Disjoint Scope Funs GFuns σ c genv Γ FVs S xs xs' C S' :
+  Lemma project_vars_Disjoint Scope Funs GFuns c genv Γ FVs S xs xs' C S' :
     Disjoint _ S (Union var Scope
                         (Union var (Funs :|: GFuns)
                                (Union var (FromList FVs) (Singleton var Γ)))) ->      
-    project_vars clo_tag Scope Funs GFuns σ c genv Γ FVs S xs xs' C S' ->
+    project_vars clo_tag Scope Funs GFuns c genv Γ FVs S xs xs' C S' ->
     Disjoint _ S (FromList xs).
   Proof.
     revert xs' C S S'; induction xs; intros xs' C S S' Hd Hproj.
@@ -1274,105 +1053,95 @@ Section Closure_conversion_util.
     - inv Hproj. rewrite FromList_cons. 
       eapply Union_Disjoint_r.
       eapply Disjoint_Singleton_r. eapply project_var_not_In; eauto.
-      inv H10.
+      inv H9.
       + eapply IHxs; [| eassumption ]. eauto.
       + assert (Hd1 : Disjoint _ (Setminus var S (Singleton var y'))
                                (FromList xs))
           by (eapply IHxs; eauto with Ensembles_DB).
-        eapply project_vars_In_Union in H14.
+        eapply project_vars_In_Union in H13.
         eapply Disjoint_Included_r. eassumption.
         eauto 10 with Ensembles_DB.
       + assert (Hd1 : Disjoint _  (S \\ [set y'] \\ [set g_env])
                                (FromList xs))
           by (eapply IHxs; eauto with Ensembles_DB).
-        eapply project_vars_In_Union in H14.
+        eapply project_vars_In_Union in H13.
         eapply Disjoint_Included_r. eassumption.
         eauto 10 with Ensembles_DB.
       + assert (Hd1 : Disjoint _ (Setminus var S (Singleton var y'))
                                (FromList xs))
           by (eapply IHxs; eauto with Ensembles_DB).
-        eapply project_vars_In_Union in H14.
+        eapply project_vars_In_Union in H13.
         eapply Disjoint_Included_r. eassumption.
         eauto 10 with Ensembles_DB.
   Qed.
 
   (** Properties about context sizes *)
 
-  Lemma project_var_sizeOf_ctx_exp (Scope Funs GFuns : Ensemble var) (σ : var -> var) 
+  Lemma project_var_sizeOf_ctx_exp (Scope Funs GFuns : Ensemble var)
         (c : ctor_tag) genv (Γ : var) (FVs : list var) (S : Ensemble var) 
     (x x' : var) (C : exp_ctx) (S' : Ensemble var) :
-    project_var clo_tag Scope Funs GFuns σ c genv Γ FVs S x x' C S' ->
+    project_var clo_tag Scope Funs GFuns c genv Γ FVs S x x' C S' ->
     sizeOf_exp_ctx C <= 4. 
   Proof.
     intros Hctx. inv Hctx; eauto.
   Qed.
   
-  Lemma project_vars_sizeOf_ctx_exp (Scope Funs GFuns : Ensemble var) (σ : var -> var) 
+  Lemma project_vars_sizeOf_ctx_exp (Scope Funs GFuns : Ensemble var)
     (c : ctor_tag) genv (Γ : var) (FVs : list var) (S : Ensemble var) 
     (xs xs' : list var) (C : exp_ctx) (S' : Ensemble var)  :
-    project_vars clo_tag Scope Funs GFuns σ c genv Γ FVs S xs xs' C S' ->
+    project_vars clo_tag Scope Funs GFuns c genv Γ FVs S xs xs' C S' ->
     sizeOf_exp_ctx C <= 4 * length xs. 
   Proof.
     intros Hctx. induction Hctx; eauto.
     rewrite sizeOf_exp_ctx_comp_ctx. simpl.
-    specialize (project_var_sizeOf_ctx_exp _ _ _ _ _ _ _ _ _ _ _ _ _ H).
+    specialize (project_var_sizeOf_ctx_exp _ _ _ _ _ _ _ _ _ _ _ _ H).
     omega.
   Qed.
 
-  Lemma make_closures_sizeOf_ctx_exp (B : fundefs) (S : Ensemble var) (Γ : var)
-        (C : exp_ctx) (σ  : var -> var) (S' : Ensemble var) :
-    make_closures clo_tag B S Γ C σ S' ->
-    sizeOf_exp_ctx C <= 3 * numOf_fundefs B.
-  Proof.
-    induction 1; eauto.
-    simpl. specialize (sizeOf_exp_grt_1 e).
-    omega.
-  Qed.
-
-  Lemma Closure_conversion_fundefs_numOf_fundefs Funs (GFuns : Ensemble var) (σ : var -> var) (c : ctor_tag) 
+  Lemma Closure_conversion_fundefs_numOf_fundefs Funs (GFuns : Ensemble var) (c : ctor_tag) 
         (FVs : list var) (B1 B2 : fundefs) :
-    Closure_conversion_fundefs clo_tag Funs GFuns σ c FVs B1 B2 ->
+    Closure_conversion_fundefs clo_tag Funs GFuns c FVs B1 B2 ->
     numOf_fundefs B1 = numOf_fundefs B2.
   Proof.
     intros Hcc; induction Hcc; eauto; simpl. congruence.
   Qed.
 
-  Lemma project_var_tag_inv Scope GFuns Funs σ c1 c2 genv Γ  S x x' C S' :
-    project_var clo_tag Scope GFuns Funs σ c1 genv Γ [] S x  x' C S' ->
-    project_var clo_tag Scope GFuns Funs σ c2 genv Γ [] S x  x' C S'.
+  Lemma project_var_tag_inv Scope GFuns Funs c1 c2 genv Γ  S x x' C S' :
+    project_var clo_tag Scope GFuns Funs c1 genv Γ [] S x  x' C S' ->
+    project_var clo_tag Scope GFuns Funs c2 genv Γ [] S x  x' C S'.
   Proof.
     intros Hc; inv Hc; (try constructor; eauto).
     inv H2.
   Qed.
 
-  Lemma project_vars_tag_inv Scope GFuns Funs σ c1 c2 genv Γ  S x x' C S' :
-    project_vars clo_tag Scope GFuns Funs σ c1 genv Γ [] S x  x' C S' ->
-    project_vars clo_tag Scope GFuns Funs σ c2 genv Γ [] S x  x' C S'.
+  Lemma project_vars_tag_inv Scope GFuns Funs c1 c2 genv Γ  S x x' C S' :
+    project_vars clo_tag Scope GFuns Funs c1 genv Γ [] S x  x' C S' ->
+    project_vars clo_tag Scope GFuns Funs c2 genv Γ [] S x  x' C S'.
   Proof.
-    revert Scope GFuns Funs σ c1 c2 Γ  S x' C S'; induction x;
-      intros Scope GFuns Funs σ c1 c2 Γ  S x' C S' Hvs; inv Hvs; try (constructor; eauto).
+    revert Scope GFuns Funs c1 c2 Γ  S x' C S'; induction x;
+      intros Scope GFuns Funs c1 c2 Γ  S x' C S' Hvs; inv Hvs; try (constructor; eauto).
     econstructor. eapply project_var_tag_inv. eassumption.
     eapply IHx; eassumption.
   Qed.
 
-  Lemma Closure_conversion_tag_inv Scope Funs GFuns g c1 c2 genv Γ e e' C :
-    Closure_conversion clo_tag Scope Funs GFuns g c1 genv Γ [] e e' C ->
-    Closure_conversion clo_tag Scope Funs GFuns g c2 genv Γ [] e e' C.
+  Lemma Closure_conversion_tag_inv Scope Funs GFuns c1 c2 genv Γ e e' C :
+    Closure_conversion clo_tag Scope Funs GFuns c1 genv Γ [] e e' C ->
+    Closure_conversion clo_tag Scope Funs GFuns c2 genv Γ [] e e' C.
   Proof.
-    revert Scope Funs GFuns g c1 c2 genv Γ e' C; induction e using exp_ind';
-      intros Scope Funs GFuns g c1 c2 genv Γ e' C Hcc; inv Hcc;
+    revert Scope Funs GFuns c1 c2 genv Γ e' C; induction e using exp_ind';
+      intros Scope Funs GFuns c1 c2 genv Γ e' C Hcc; inv Hcc;
         try (econstructor; eauto; eapply project_vars_tag_inv; eassumption);
         try (econstructor; eauto; eapply project_var_tag_inv; eassumption).
     - econstructor; eauto.
-      eapply project_var_tag_inv. eassumption. inv H13.
+      eapply project_var_tag_inv. eassumption. inv H12.
       constructor.
     - econstructor; eauto.
       eapply project_var_tag_inv. eassumption.
-      inv H13. destruct H2 as [Heq [C' [e' [HeqC Hcc']]]].
+      inv H12. destruct H2 as [Heq [C' [e' [HeqC Hcc']]]].
       destruct y as [c2' e2]. simpl in *; subst.
       constructor; eauto.
       split; eauto. do 2 eexists; split; eauto. simpl. reflexivity.
-      assert (Hcc1 : Closure_conversion clo_tag Scope Funs GFuns g c2 genv Γ [] (Ecase v l) (Ecase x' l') C).
+      assert (Hcc1 : Closure_conversion clo_tag Scope Funs GFuns c2 genv Γ [] (Ecase v l) (Ecase x' l') C).
       { eapply IHe0. econstructor; eauto. }
       inv Hcc1. eassumption.
   Qed.
